theories/iris/runtime.v
@@ -28,9 +28,9 @@ Section Runtime.
            lp_host := fun _ _ _ _ => False |}.
 
   Definition spec_alloc_gc (cl : function_closure) : Prop :=
-    forall ps sz pm fr,
+    forall θ sz pm fr,
       let ks := kinds_of_pointer_map pm (Wasm_int.nat_of_uint i32m sz) in
-      rt_token rti sr ps -∗
+      rt_token rti sr θ -∗
       N.of_nat sr.(sr_func_alloc_gc) ↦[wf] cl -∗
       ↪[frame] fr -∗
       ↪[RUN] -∗
@@ -46,7 +46,7 @@ Section Runtime.
                  ∃ θ' ℓ a ws,
                    ⌜vs = [VAL_int32 (Wasm_int.int_of_Z i32m a)]⌝ ∗
                      ⌜repr_location θ' ℓ a⌝ ∗
-                     rt_token rti sr (ps <| ps_gc_ptrs := θ' |>) ∗
+                     rt_token rti sr θ' ∗
                      ℓ ↦gcl ks ∗
                      ℓ ↦gco ws;
            lp_trap := True;
@@ -61,9 +61,9 @@ Section Runtime.
     True.
 
   Definition spec_registerroot (cl : function_closure) : Prop :=
-    forall ps ℓ a fr,
-      repr_location ps.(ps_gc_ptrs) ℓ (Wasm_int.Z_of_uint i32m a) ->
-      rt_token rti sr ps -∗
+    forall θ ℓ a fr,
+      repr_location θ ℓ (Wasm_int.Z_of_uint i32m a) ->
+      rt_token rti sr θ -∗
       N.of_nat sr.(sr_func_registerroot) ↦[wf] cl -∗
       ↪[RUN] -∗
       ↪[frame] fr -∗
@@ -76,8 +76,7 @@ Section Runtime.
                  N.of_nat sr.(sr_func_registerroot) ↦[wf] cl ∗
                  ∃ a',
                    ⌜vs = [VAL_int32 (Wasm_int.int_of_Z i32m (Z.of_N a'))]⌝ ∗
-                   (* TODO: Specifying ps_gc_roots seems redundant with ↦gcr? *)
-                   rt_token rti sr (ps <| ps_gc_roots ::= ({[a']} ∪.) |>) ∗
+                   rt_token rti sr θ ∗
                    a' ↦gcr ℓ;
            lp_trap := True;
            lp_br := fun _ _ => False;
@@ -85,8 +84,8 @@ Section Runtime.
            lp_host := fun _ _ _ _ => False |}.
 
   Definition spec_unregisterroot (cl : function_closure) : Prop :=
-    forall ps ℓ a fr,
-      rt_token rti sr ps -∗
+    forall θ ℓ a fr,
+      rt_token rti sr θ -∗
       Wasm_int.N_of_uint i32m a ↦gcr ℓ -∗
       N.of_nat sr.(sr_func_unregisterroot) ↦[wf] cl -∗
       ↪[RUN] -∗
@@ -98,11 +97,8 @@ Section Runtime.
              fun vs =>
                ↪[RUN] ∗
                  N.of_nat sr.(sr_func_unregisterroot) ↦[wf] cl ∗
-                 (* TODO: Specifying ps_gc_roots seems redundant with ↦gcr? *)
-                 rt_token rti sr (ps <| ps_gc_roots ::= ({[Wasm_int.N_of_uint i32m a]} ∖.) |>) ∗
-                 ∃ a',
-                   ⌜vs = [VAL_int32 (Wasm_int.int_of_Z i32m a')]⌝ ∗
-                     ⌜repr_location ps.(ps_gc_ptrs) ℓ a'⌝;
+                 rt_token rti sr θ ∗
+                 ∃ a', ⌜vs = [VAL_int32 (Wasm_int.int_of_Z i32m a')]⌝ ∗ ⌜repr_location θ ℓ a'⌝;
            lp_trap := True;
            lp_br := fun _ _ => False;
            lp_ret := fun _ => False;
